src/examples/GPU.Example1.fst
@@ -26,7 +26,7 @@ fn main (_:unit)
   let gr = gpu_alloc0 #u64 ();
    
   Box.to_ref_pts_to r;
-  GPU.Ref.gpu_memcpy_host_to_device (Box.box_to_ref r) gr;
+  GPU.Ref.gpu_memcpy_host_to_device gr (Box.box_to_ref r);
 
   launch_kernel_1 (fun () -> kernel gr #(hide 1uL));
 
