src/examples/matmul-tile/GPU.MatMulTile.fst
@@ -131,8 +131,8 @@ fn main
   let ga1 = gpu_array_alloc #u64 (Kernel.rows *^ Kernel.shared);
   let ga2 = gpu_array_alloc #u64 (Kernel.shared *^ Kernel.columns);
 
-  GPU.Array.gpu_memcpy_host_to_device a1 ga1 (Kernel.rows *^ Kernel.shared);
-  GPU.Array.gpu_memcpy_host_to_device a2 ga2 (Kernel.shared *^ Kernel.columns);
+  GPU.Array.gpu_memcpy_host_to_device ga1 a1 (Kernel.rows *^ Kernel.shared);
+  GPU.Array.gpu_memcpy_host_to_device ga2 a2 (Kernel.shared *^ Kernel.columns);
 
   let gr = gpu_array_alloc #u64 size;
 
